\documentclass{article}
\usepackage{epsfig}
% Packages requested by user
\usepackage{amssymb}
\usepackage{amsmath}

\pagestyle{empty}
\begin{document}
$(x,y,r)$
\pagebreak

$r$
\pagebreak

$d\pm\epsilon$
\pagebreak

$ f $
\pagebreak

\[ f(0) + f'(0) x + \frac{f''(0)}{2} x^2 + \frac{f'''(0)}{3!} x^3 + \cdots \]
\pagebreak

$ f(x) $
\pagebreak

\[ f(M) = f(0) + f'(0) M + \frac{f''(0)}{2} M^2 + \frac{f'''(0)}{3!} M^3 + \cdots \]
\pagebreak

$ \cos(M) $
\pagebreak

$ \cosh(M) $
\pagebreak

$ M $
\pagebreak

\[ \exp(M) = \sum_{k=0}^\infty \frac{M^k}{k!}. \]
\pagebreak

$ y' = My $
\pagebreak

$ y(0) = y_0 $
\pagebreak

$ y(t) = \exp(M) y_0 $
\pagebreak

$ 20 n^3 $
\pagebreak

$ n $
\pagebreak

\[ \exp \left[ \begin{array}{ccc} 0 & \frac14\pi & 0 \\ -\frac14\pi & 0 & 0 \\ 0 & 0 & 0 \end{array} \right] = \left[ \begin{array}{ccc} \frac12\sqrt2 & -\frac12\sqrt2 & 0 \\ \frac12\sqrt2 & \frac12\sqrt2 & 0 \\ 0 & 0 & 1 \end{array} \right]. \]
\pagebreak

$ \frac14\pi $
\pagebreak

$ X $
\pagebreak

$ \exp(X) = M $
\pagebreak

$ (-\pi,\pi] $
\pagebreak

\[ \log \left[ \begin{array}{ccc} \frac12\sqrt2 & -\frac12\sqrt2 & 0 \\ \frac12\sqrt2 & \frac12\sqrt2 & 0 \\ 0 & 0 & 1 \end{array} \right] = \left[ \begin{array}{ccc} 0 & \frac14\pi & 0 \\ -\frac14\pi & 0 & 0 \\ 0 & 0 & 0 \end{array} \right]. \]
\pagebreak

$ M^p $
\pagebreak

$ \exp(p \log(M)) $
\pagebreak

$ (-1, 1) $
\pagebreak

$ T $
\pagebreak

\[ T = \left[ \begin{array}{cc} T_1 & T_2 \\ 0 & 0 \end{array} \right] \]
\pagebreak

$ T_1 $
\pagebreak

$ T^p $
\pagebreak

\[ T^p = \left[ \begin{array}{cc} T_1^p & T_1^{-1} T_1^p T_2 \\ 0 & 0 \end{array}. \right] \]
\pagebreak

\[ \left[ \begin{array}{ccc} \cos1 & -\sin1 & 0 \\ \sin1 & \cos1 & 0 \\ 0 & 0 & 1 \end{array} \right]^{\frac14\pi} = \left[ \begin{array}{ccc} \frac12\sqrt2 & -\frac12\sqrt2 & 0 \\ \frac12\sqrt2 & \frac12\sqrt2 & 0 \\ 0 & 0 & 1 \end{array} \right]. \]
\pagebreak

$ f^{(n)}(x) $
\pagebreak

$ \sin(M) $
\pagebreak

$ \sinh(M) $
\pagebreak

$ M^{1/2} $
\pagebreak

$ S = M^{1/2} $
\pagebreak

$ S^2 = M $
\pagebreak

$ 25 n^3 $
\pagebreak

$ 3\frac13 n^3 $
\pagebreak

$ (-\frac12\pi, \frac12\pi] $
\pagebreak

\[ \left[ \begin{array}{cc} \cos(\frac13\pi) & -\sin(\frac13\pi) \\ \sin(\frac13\pi) & \cos(\frac13\pi) \end{array} \right], \]
\pagebreak

\[ \left[ \begin{array}{cc} \cos(\frac16\pi) & -\sin(\frac16\pi) \\ \sin(\frac16\pi) & \cos(\frac16\pi) \end{array} \right]. \]
\pagebreak

$ a_i $
\pagebreak

$ p(x) = a_0 + a_{1}x + ... + a_{n-1}x^{n-1} + x^n $
\pagebreak

$ p $
\pagebreak

$ p(x) = (x-r_1)(x-r_2)...(x-r_n) $
\pagebreak

$C(p)$
\pagebreak

$ \forall r_i $
\pagebreak

$ p(x) = \sum_{k=0}^d a_k x^k $
\pagebreak

$ |r_i| \le C(p) = \sum_{k=0}^{d} \left | \frac{a_k}{a_d} \right | $
\pagebreak

$a_d \neq 0$
\pagebreak

$c(p)$
\pagebreak

$ \forall r_i \neq 0 $
\pagebreak

$ |r_i| \ge c(p) = \left( \sum_{k=0}^{d} \left | \frac{a_k}{a_0} \right | \right)^{-1} $
\pagebreak

$ p(x) = a_0 + a_1 x + a_2 x^2 + a_{3} x^3 + x^4 $
\pagebreak

$ \left [ \begin{array}{cccc} 0 & 0 & 0 & a_0 \\ 1 & 0 & 0 & a_1 \\ 0 & 1 & 0 & a_2 \\ 0 & 0 & 1 & a_3 \end{array} \right ] $
\pagebreak

$r_1,r_2,...,r_d$
\pagebreak

$ \forall i,j \in [1;d],~ \| r_i \| \neq \| r_j \| $
\pagebreak

$ k $
\pagebreak

$ A $
\pagebreak

$ V $
\pagebreak

$ A V = D V $
\pagebreak

$ A V = D B V $
\pagebreak

$ A = V D V^{-1} $
\pagebreak

$ A^{1/2} = V D^{1/2} V^{-1} $
\pagebreak

$ V D^{-1/2} V^{-1} $
\pagebreak

$ CINV = (C * C^T)^{-1} * C $
\pagebreak

$ 1/2((Ax).x) - bx $
\pagebreak

$ Cx \le f $
\pagebreak

$ 2^{-s} $
\pagebreak

$ (V+U)(V-U)^{-1} $
\pagebreak

$ \exp(A) $
\pagebreak

$ A = 0 $
\pagebreak

$ s $
\pagebreak

$ 2^{-s} x $
\pagebreak

$ \exp(2^{-\mbox{squarings}}M) $
\pagebreak

$ M = 0 $
\pagebreak

\[ \sum_{k=i}^m A_{ik} X_{kj} + \sum_{k=1}^j X_{ik} B_{kj} = C_{ij}. \]
\pagebreak

\[ X_{ij} = \frac{1}{A_{ii} + B_{jj}} \Bigl( C_{ij} - \sum_{k=i+1}^m A_{ik} X_{kj} - \sum_{k=1}^{j-1} X_{ik} B_{kj} \Bigr). \]
\pagebreak

$ i=m,\ldots,1 $
\pagebreak

$ j=1,\ldots,n $
\pagebreak

$ A^p $
\pagebreak

$ \exp(p \log(A)) $
\pagebreak

$ 1 + 3x^2 $
\pagebreak

$ [ 1, 0, 3 ] $
\pagebreak

$ |x| \le 1 $
\pagebreak

$ 3 + x^2 $
\pagebreak

$ [ 3, 0, 1 ] $
\pagebreak

\begin{align*} C(u) & = \sum_{i=0}^{n}N_{i,p}(u)P_i \end{align*}
\pagebreak

$u$
\pagebreak

\begin{align*} C(u) & = \sum_{i=0}^{n}N_{i,p}P_i \end{align*}
\pagebreak

$u \in [0;1]$
\pagebreak

\begin{align*} \frac{d^i}{du^i}C(u) & = \sum_{i=0}^{n} \frac{d^i}{du^i} N_{i,p}(u)P_i \end{align*}
\pagebreak

$p+1$
\pagebreak

$P_i$
\pagebreak

$p$
\pagebreak

\begin{align*} N_{i,p}(u), \hdots, N_{i+p+1,p}(u) \end{align*}
\pagebreak

\begin{align*} \frac{d^i}{du^i} N_{i,p}(u), \hdots, \frac{d^i}{du^i} N_{i+p+1,p}(u) \end{align*}
\pagebreak

\begin{align*} u_0 & = \hdots = u_p = 0 \\ u_{m-p} & = \hdots = u_{m} = 1 \\ u_{j+p} & = \frac{1}{p}\sum_{i=j}^{j+p-1}\bar{u}_i \quad\quad j=1,\hdots,n-p \end{align*}
\pagebreak

$m+1$
\pagebreak

\end{document}
